viper-total-heaps/PaperResults.thy
@@ -26,9 +26,9 @@ text \<open>Whenever a ctrl-click takes you to another theory, you can use the g
       You can also use the "Sidekick" view on the right side of the Isabelle IDE to quickly jump to a section or 
       subsection.\<close>
 
-section \<open>2: "Viper and Boogie: Background and Semantics"\<close>
+section \<open>2 Viper and Boogie: Background and Semantics\<close>
 
-subsection \<open>2.1: The Viper and Boogie languages\<close>
+subsection \<open>2.1 The Viper and Boogie languages\<close>
 
 text \<open>The Viper AST for statements is defined in \<^typ>\<open>ViperLang.stmt\<close>.
       The Boogie AST for statements is defined in \<^typ>\<open>Ast.bigblock\<close>\<close>
@@ -49,7 +49,7 @@ text \<open> \<^item> Statement single step reduction is defined via \<^const>\<
   where \<open>\<Gamma>\<^sub>v\<close> captures both \<^term>\<open>P\<close> and \<^term>\<open>ctxt\<close>.
  \<close>
 
-subsection \<open>2.3: Viper Semantics\<close>
+subsection \<open>2.3 Viper Semantics\<close>
 
 paragraph \<open>Viper states\<close>
 text \<open>Viper outcomes are defined in \<^typ>\<open>'a stmt_result_total\<close>.
@@ -71,8 +71,8 @@ text \<open>The big-step judgement for Viper statements is defined via \<^const>
       in state \<open>\<sigma>\<^sub>v\<close>) corresponds to \<^prop>\<open>red_stmt_total ctxt R \<Lambda> s \<sigma>\<^sub>v r\<^sub>v\<close> in the formalisation,
       where the Viper context \<^term>\<open>\<Gamma>\<^sub>v\<close> captures both \<^term>\<open>ctxt\<close> and \<^term>\<open>\<Lambda>\<close>
 
-      The parameter \<^term>\<open>R\<close> is not required for the Viper subset in the paper. In our proofs, 
-      it is always instantiated as \<open>\<lambda>_. True\<close>.
+      The parameter \<^term>\<open>R\<close> is not required for the Viper subset in the paper. In our generated proofs, 
+      it is always instantiated as \<^term>\<open>\<lambda>_. True\<close>.
 \<close>
 
 paragraph \<open>Viper expression evaluation\<close>
@@ -84,7 +84,7 @@ text \<open>The expression evaluation is defined via \<^const>\<open>red_pure_ex
       corresponds to \<^prop>\<open>ctxt, R, Some(\<sigma>\<^sub>v) \<turnstile> \<langle>e; \<sigma>\<^sub>v\<rangle> [\<Down>]\<^sub>t VFailure\<close>.
 
       As for the statement reduction, \<^term>\<open>R\<close> is not required for the Viper subset in the paper and is always
-      instantiated as \<open>\<lambda>_. True\<close> in our proofs. \<^term>\<open>ctxt\<close> is the same as for the statement reduction
+      instantiated as \<^term>\<open>\<lambda>_. True\<close> in our generated proofs. \<^term>\<open>ctxt\<close> is the same as for the statement reduction
       but is redundant for the Viper subset in the paper and thus was omitted in the presentation.      
 
       One difference to the paper, is that the expression evaluation in the formalisation takes two 
@@ -92,7 +92,7 @@ text \<open>The expression evaluation is defined via \<^const>\<open>red_pure_ex
       outside of the subset of the paper and that's why in the paper we present the evaluation just with one 
       state to ease the presentation.
        
-      In almost all cases of the semantics, these two states are chosen to be the same one and thus 
+      In almost all cases of the semantics formalisation, these two states are chosen to be the same one and thus 
       directly correspond to the paper. The only case where the two states differ is during \<open>remcheck\<close> operations, 
       where one state is instantiated to be the \<^emph>\<open>reduction state\<close> and the other the \<^emph>\<open>expression evaluation state\<close>
       (introduced on lines 312-317 in the paper). The expression evaluation checks whether there
@@ -110,6 +110,8 @@ paragraph \<open>Exhale semantics\<close>
 text \<open>The rule (EXH-SUCC) is given by:\<close>
 
 lemmas EXH_SUCC = RedExhale \<comment>\<open>Note: you can ctrl-click on \<open>RedExhale\<close> to jump to the rule\<close>
+
+text \<open>TODO: discuss why nonDetSelect is the same as \<^const>\<open>havoc_locs_state\<close>\<close>
 
 text \<open>The rule (EXH-FAIL) is given by:\<close>
 
@@ -134,6 +136,50 @@ text \<open>The statement reduction rule for \<open>inhale\<close> is given by:\
 lemmas red_inhale = RedInhale
 
 text \<open>This rule is defined via a helper definition \<^const>\<open>red_inhale\<close>.\<close>
+
+
+section \<open>3 A Forward Simulation Methodology For Front-End Translations\<close>
+
+subsection \<open>3.2 One Simulation Judgement to Rule Them All\<close>
+
+text \<open>The generic forward simulation judgement \<open>sim\<close> in the paper is defined in \<^const>\<open>rel_general\<close>.
+      The notation \<open>sim\<^sub>\<Gamma>\<^sub>b(R\<^sub>i\<^sub>n, R\<^sub>o\<^sub>u\<^sub>t, Succ, Fail, \<gamma>\<^sub>i\<^sub>n, \<gamma>\<^sub>o\<^sub>u\<^sub>t)\<close> corresponds to
+      \<^prop>\<open>rel_general R\<^sub>i\<^sub>n R\<^sub>o\<^sub>u\<^sub>t Succ Fail P ctxt \<gamma>\<^sub>i\<^sub>n \<gamma>\<^sub>o\<^sub>u\<^sub>t\<close>, where the Boogie context \<open>\<Gamma>\<^sub>b\<close> captures both
+      \<^term>\<open>P\<close> and \<^term>\<open>ctxt\<close>.\<close>
+
+paragraph \<open>Three common instantiations of \<open>sim\<close>\<close>
+text \<open>For the three common instantiations shown at the bottom of figure 4, in the formalisation,
+      the Boogie context \<open>\<Gamma>\<^sub>b\<close> captures both \<^term>\<open>P\<close> and \<^term>\<open>ctxt\<close>, the Viper context \<open>\<Gamma>\<^sub>v\<close> captures 
+      both \<^term>\<open>ctxt_vpr\<close> and \<^term>\<open>\<Lambda>\<close>, and \<^term>\<open>StateCons\<close> corresponds to parameter \<^term>\<open>R\<close> discussed
+      above for the statement and expression reduction and is always instantiated to be \<^term>\<open>\<lambda>_.True\<close>
+      in our generated proofs.\<close>
+
+text \<open>The statement simulation is defined in \<^const>\<open>stmt_rel\<close>. The notation
+     \<open>stmSim\<^sub>\<Gamma>\<^sub>v,\<^sub>\<Gamma>\<^sub>b(R\<^sub>i\<^sub>n, R\<^sub>o\<^sub>u\<^sub>t, s, \<gamma>\<^sub>i\<^sub>n, \<gamma>\<^sub>o\<^sub>u\<^sub>t)\<close> in the paper corresponds to 
+     \<^prop>\<open>stmt_rel R\<^sub>i\<^sub>n R\<^sub>o\<^sub>u\<^sub>t ctxt_vpr StateCons \<Lambda> P ctxt s \<gamma>\<^sub>i\<^sub>n \<gamma>\<^sub>o\<^sub>u\<^sub>t\<close> in the formalisation.\<close>
+
+text \<open>The remcheck simulation is defined in \<^const>\<open>exhale_rel0\<close>. The notation
+     \<open>rcSim\<^sub>\<Gamma>\<^sub>b(R\<^sub>i\<^sub>n, R\<^sub>o\<^sub>u\<^sub>t, A, \<gamma>\<^sub>i\<^sub>n, \<gamma>\<^sub>o\<^sub>u\<^sub>t)\<close> in the paper corresponds to 
+      \<^prop>\<open>exhale_rel0 R\<^sub>i\<^sub>n R\<^sub>o\<^sub>u\<^sub>t ctxt_vpr StateCons P ctxt A \<gamma>\<^sub>i\<^sub>n \<gamma>\<^sub>o\<^sub>u\<^sub>t\<close> in the formalisation.
+     For convenience reasons, \<^term>\<open>R\<^sub>i\<^sub>n\<close> and \<^term>\<open>R\<^sub>o\<^sub>u\<^sub>t\<close> are curried, and thus the instantiation via
+     \<^const>\<open>rel_general\<close> uncurries them.
+     In our formalisation, we always directly work with a remcheck simulation that additionally takes
+     a predicate \<open>Q\<close> on assertions as a parameter as described in Section 3.5 of the paper.
+     The notation \<open>rcSim\<^sub>\<Gamma>\<^sub>b\<^sup>Q(R\<^sub>i\<^sub>n, R\<^sub>o\<^sub>u\<^sub>t, A, \<gamma>\<^sub>i\<^sub>n, \<gamma>\<^sub>o\<^sub>u\<^sub>t)\<close> in the paper (Figure 7) corresponds to 
+     \<^prop>\<open>exhale_rel R\<^sub>i\<^sub>n R\<^sub>o\<^sub>u\<^sub>t Q ctxt_vpr StateCons P ctxt A \<gamma>\<^sub>i\<^sub>n \<gamma>\<^sub>o\<^sub>u\<^sub>t\<close>.
+    
+     \<^const>\<open>exhale_rel\<close> is directly defined in terms of the generic simulation judgement, but the following
+     lemma shows that this is equivalent to defining \<^const>\<open>exhale_rel\<close> in terms \<^const>\<open>exhale_rel0\<close>
+     as we do in the paper for the sake of presentation:
+\<close>
+
+lemma exhale_rel_exhale_rel0_inst_equiv: 
+  "exhale_rel R\<^sub>i\<^sub>n R\<^sub>o\<^sub>u\<^sub>t Q ctxt_vpr StateCons P ctxt A \<gamma> \<gamma>' \<longleftrightarrow>
+   exhale_rel0 (\<lambda>\<omega>def \<omega> ns. R\<^sub>i\<^sub>n \<omega>def \<omega> ns \<and> Q A \<omega>def \<omega>) R\<^sub>o\<^sub>u\<^sub>t ctxt_vpr StateCons P ctxt A \<gamma> \<gamma>'"
+  unfolding exhale_rel_def exhale_rel0_def
+  by simp
+
+
 
 end
 
